cleanup

Lampe/Lampe/Tactic/Traits.lean
@@ -5,107 +5,154 @@ import Lampe.Syntax
 
 open Lean Elab.Tactic Parser.Tactic Lean.Meta Qq
 
-def applyImpl (goal : MVarId) (impl : TSyntax `term) (generics : List $ TSyntax `term) : TacticM $ List MVarId := do
-  let generics ← Lampe.mkHListLit generics
-  let newGoals ← evalTacticAt (←`(tactic|
-    apply Lampe.TraitResolution.ok (impl := $impl) (implGenerics := $generics) (h_mem := by try tauto) <;> (first | rfl | tauto)
-  )) goal
-  pure newGoals
+partial def extractImpl (expr : Lean.Expr) : TacticM $ TSyntax `term := do
+  match_expr expr with
+  | Prod.mk _ _ _name impl => return ← impl.toSyntax
+  | _ => throwError "Didn't expect that..."
 
-def tryImpls (allImpls : List $ TSyntax `term) (generics : List $ TSyntax `term) : TacticM Unit := do
+partial def extractAllImpls (envExpr : Expr) : TacticM $ List (TSyntax `term) := do
+  let traitsListExpr ← mkAppM `Lampe.Env.traits #[envExpr]
+  let reducedTraitsListExpr ← withAtLeastTransparency .all <| whnf traitsListExpr
+
+  let rec go (listExpr : Expr) : TacticM $ List (TSyntax `term) := do
+    dbg_trace "-------------------------------"
+    dbg_trace "RUNNING ON: listExpr {listExpr}"
+    dbg_trace "-------------------------------"
+
+    let currentExpr ← withAtLeastTransparency .all <| whnf listExpr
+    if currentExpr.isAppOfArity ``List.cons 3 then
+      dbg_trace "CONS CASE"
+      let args := currentExpr.getAppArgs
+      let headExpr ← whnf args[1]! -- head
+      let tailExpr := args[2]! -- tail
+      if headExpr.isAppOfArity ``Prod.mk 4 then
+        dbg_trace "EXTRACTING : {headExpr}"
+        let implSyntax ← extractImpl headExpr
+        let restImpls ← go tailExpr
+        return implSyntax :: restImpls
+      else
+        throwError s!"extractAllImpls: expected Prod.mk in List.cons, got {headExpr}"
+    else if currentExpr.isAppOfArity ``List.nil 1 then
+      dbg_trace "NIL CASE"
+      return []
+    else if currentExpr.isAppOfArity ``List.append 3 then
+      dbg_trace "APPEND CASE"
+      let args := currentExpr.getAppArgs
+      let list1Expr := args[1]! -- first list
+      let list2Expr := args[2]! -- second list
+      let impls1 ← go list1Expr
+      let impls2 ← go list2Expr
+      return impls1 ++ impls2
+    else if currentExpr.isSorry then
+      dbg_trace s!"extractAllImpls: encountered sorry at {currentExpr}, treating as empty list part."
+      return []
+    else
+      throwError s!"extractAllImpls: unhandled expression form {currentExpr}"
+
+  go reducedTraitsListExpr
+
+def trait1 : Lampe.TraitImpl := sorry
+def trait2 : Lampe.TraitImpl := sorry
+def trait3 : Lampe.TraitImpl := sorry
+def trait4 : Lampe.TraitImpl := sorry
+def trait5 : Lampe.TraitImpl := sorry
+def trait6 : Lampe.TraitImpl := sorry
+def trait7 : String × Lampe.TraitImpl := ("Trait7", trait6)
+
+
+def env1 : Lampe.Env := ⟨[], [("Trait1", trait1), ("Trait2", trait2)]⟩
+def env2 : Lampe.Env := ⟨[], [("Trait3", trait3), ("Trait4", trait4)]⟩
+def env3 : Lampe.Env := ⟨[], [trait7]⟩
+def env4 : Lampe.Env := ⟨[], [("Trait5", trait5)]⟩
+def env5 := env4
+def env6 := env5
+
+def env7 := env1 ++ env2 ++ env3 ++ env6
+
+elab "testing" env:term : tactic => do
+  let xs ← extractAllImpls (← elabTerm env none)
+  dbg_trace "ALL OF THE REST: {← xs.mapM $ (elabTerm · none)}"
+  return ()
+
+example : Prop := by
+  testing env7
+  sorry
+
+open Lampe in
+theorem callTrait_direct_intro {impls : List $ Lampe.Ident × Function}
+    (h_trait : TraitResolution Γ ⟨⟨traitName, traitKinds, traitGenerics⟩, selfTp⟩ impls)
+    (h_fn : impls.find? (fun (n, _) => n = fnName) = some (fnName, func))
+    (hkc : func.generics = kinds)
+    (htci : (func.body _ (hkc ▸ generics) |>.argTps) = argTps)
+    (htco : (func.body _ (hkc ▸ generics) |>.outTp) = outTp)
+    (h_hoare: STHoare p Γ H (htco ▸ (func.body _ (hkc ▸ generics) |>.body (htci ▸ args))) Q) :
+    STHoare p Γ H (Expr.call argTps outTp (.trait (some selfTp) traitName traitKinds traitGenerics fnName kinds generics) args) Q := by
+  apply STHoare.callTrait_intro (selfTp := selfTp) (traitName := traitName) (traitKinds := traitKinds) (traitGenerics := traitGenerics) (fnName := fnName) (outTp := outTp) (generics := generics)
+  · simp [SLP.entails_top]
+  · exact h_trait
+  · simp only [Option.eq_some_iff_get_eq] at h_fn
+    cases h_fn
+    rename_i h
+    rw [←h]
+    simp [List.get_find?_mem]
+  · assumption
+  · assumption
+  · assumption
+
+elab "try_all_traits" "[" generics:term,* "]" env:term : tactic => do
+  let envExpr ← elabTerm env none
+  let impls ← extractAllImpls envExpr
+  let generics ← Lampe.mkHListLit generics.getElems.toList
   let oldState ← saveState
   let mainGoal ← getMainGoal
-  match allImpls with
-  | impl :: impls => do
-    let subGoals ← applyImpl mainGoal impl generics
-    if subGoals.length > 0 then
-      oldState.restore
-      tryImpls impls generics
-    else
-      replaceMainGoal subGoals
-      return ()
-  | [] => throwError "no impl applies"
 
-partial def extractImpl (expr : Lean.Expr) : TacticM $ TSyntax `term := match expr with
-| .const name us => do extractImpl (← whnf (.const name us))
-| .app (.app (.app (.const `Prod.snd _) _) _) implPairExpr => extractImpl implPairExpr
-| .app (.app (.app (.app (.const `Prod.mk _) _) _) _) implExpr => extractImpl implExpr
-| .app (.app (.app (.app (.app (.app (.const `Lampe.TraitImpl.mk _) _) _) _) _) _) _ => do `($(← expr.toSyntax))
-| _ => throwError s!"failed to match with {expr} in impl extraction"
+  for impl in impls do
+    let implExpr ← elabTerm impl none
+    let implExprImpls ← whnf (← mkAppM `Lampe.TraitImpl.impl #[implExpr])
+    let funcList ← (withAtLeastTransparency .all (whnf (mkApp implExprImpls (← elabTerm generics
+    none))))
 
-partial def extractImpls (expr : Lean.Expr) : TacticM $ List (TSyntax `term) := match expr with
-  | .const name us => do extractImpls (← whnf (.const name us))
-  | .app (.const `Lampe.Env.traits _) envExpr => extractImpls envExpr
-  | .app (.app (.const `Lampe.Env.mk _) _) implsExpr => extractImpls implsExpr
-  | .app (.app (.app (.const `List.cons _) _) implExpr) rem => do
-    let implSyn ← extractImpl implExpr
-    pure (implSyn :: (← extractImpls rem))
-  | .app (.const `List.nil _) _ => pure []
-  | _ => throwError s!"failed to match with {expr} in trait extraction"
+    let (_, funcs) ← liftOption funcList.listLit?
+    dbg_trace "trying impl"
 
-def extractAllImpls (envExprs : List Expr) : TacticM $ List (TSyntax `term) :=
-  envExprs.foldlM (init := [])
-    fun acc envExpr => extractImpls envExpr >>= fun impls => pure (acc ++ impls)
+    for func in funcs do
+      dbg_trace "trying func"
+      let funcArgs := func.getAppArgs
+      let funcFunc := funcArgs.reverse[0]!
 
-partial def extractEnvs (expr : Expr) : TacticM $ List Expr := do
-  if expr.isAppOf `HAppend.hAppend then
-    let args := expr.getAppArgs
-    let env₁ := args[4]!
-    let env₂ := args[5]!
-    return (← extractEnvs env₁) ++ (← extractEnvs env₂)
+      try
+        dbg_trace "1: {(← getUnsolvedGoals).length}"
+        let callDirectGoals ← evalTacticAt (←`(tactic|
+          apply callTrait_direct_intro (func := $(←funcFunc.toSyntax))
+        )) mainGoal
 
-  let reducedExpr ← unfoldDefinition expr
-  if reducedExpr.isAppOf `Lampe.Env.mk then
-    return [expr]
-  else if reducedExpr.isAppOf `HAppend.hAppend then
-    let args := reducedExpr.getAppArgs
-    let env₁ := args[4]!
-    let env₂ := args[5]!
-    return (← extractEnvs env₁) ++ (← extractEnvs env₂)
-  else
-    throwError s!"Failed to match with {reducedExpr} in env extraction"
+        dbg_trace "2: {(← getUnsolvedGoals).length}"
+        let traitResGoal := callDirectGoals[0]!
+        let traitResGoals ← evalTacticAt (←`(tactic|
+          apply Lampe.TraitResolution.ok (impl := $impl) (implGenerics := $generics) (h_mem := by tauto)
+        )) traitResGoal
 
-syntax "apply_impl" "[" term,* "]" term : tactic
-syntax "try_impls" "[" term,* "]" "[" term,* "]" : tactic
-syntax "try_impls_all" "[" term,* "]" term : tactic
+        dbg_trace "3: {(← getUnsolvedGoals).length}"
+        for goal in callDirectGoals.drop 1 do
+          let newGoals ← evalTacticAt (← `(tactic|
+            first | try tauto | try with_unfolding_all rfl
+          )) goal
+          pushGoals newGoals
 
-/--
-`apply_impl` applies a given trait implementation `TraitImpl` to the main goal, which must be a `TraitResolution`.
+        dbg_trace "4: {(← getUnsolvedGoals).length}"
+        for goal in traitResGoals do
+          let goals ← evalTacticAt (←`(tactic| first | try tauto | with_unfolding_all rfl)) goal
+          pushGoals goals
 
-Example:
-```
-apply_impl [Tp.field] t1 -- applies `t1` with impl generics instantiated to `h![Tp.field]`
-```
--/
-elab "apply_impl" "[" generics:term,* "]" impl:term : tactic => do
-  let mainGoal ← getMainGoal
-  let newGoals ← applyImpl mainGoal impl generics.getElems.toList
-  replaceMainGoal newGoals
+        dbg_trace "5: {(← getUnsolvedGoals).length}"
+        if (← getUnsolvedGoals).length == 1 then
+          dbg_trace "Success!"
+          return
+        else
+          oldState.restore
+          dbg_trace "unsolved: {(← getUnsolvedGoals).length}"
+      catch _ =>
+        oldState.restore
 
-/--
-`try_impls` takes a comma separated sequence of `TraitImpl`s in square brackets,
-and it tries them one by one by calling `apply_impl` until one of them succeeds.
-
-Example:
-```
-try_impls [Tp.field] [t1, t2] -- tries `t1` and `t2` with impl generics instantiated to `h![Tp.field]`
-```
--/
-elab "try_impls" "[" generics:term,* "]" "[" impls:term,* "]" : tactic => do
-  tryImpls impls.getElems.toList generics.getElems.toList
-
-/--
-`try_impls_all` takes an `Lampe.Env`, and tries all the trait impls one by one to solve the main `TraitResolution` goal.
-
-Example:
-```
-def env : Lampe.Env := ⟨[], [⟨"TraitName", t1⟩, ⟨"TraitName", t2⟩]⟩
-
-try_impls_all [Tp.field] env -- tries `t1` and `t2` with impl generics instantiated to `h![Tp.field]`
-```
--/
-elab "try_impls_all" "[" generics:term,* "]" envSyn:term : tactic => do
-  let envExpr ← elabTerm envSyn none
-  let envs ← extractEnvs envExpr
-  let impls ← extractAllImpls envs
-  tryImpls impls generics.getElems.toList
+  oldState.restore
+  throwError "No trait implementation could be applied successfully"
